Page table abstraction for experimental-timeprot (#422)
* WIP on v/paddr distinction via page table abstraction, d_running proved

* Done 1st attempt page table abstraction for v/paddrs; TODO update example

* Make types work for basic test instantiation; an `id` page table for now

Signed-off-by: Scott Buckley <sbuckley@anchorage.keg.cse.unsw.edu.au>

proof/infoflow/timeprotection/MemSysExample_Generic32Bit_A.thy
@@ -44,31 +44,35 @@ begin
 (* Note: There should be "x" mask bits for an "x word" type, and the offset
    should match the number of zeroes to the right of the mask. *)
 type_synonym L1_tag_A = "22 word"
-definition L1_tag_mask :: address where "L1_tag_mask = 0b11111111111111111111110000000000"
+definition L1_tag_mask :: machine_word where "L1_tag_mask = 0b11111111111111111111110000000000"
 definition L1_tag_offset :: nat where "L1_tag_offset = 10"
 type_synonym L1_index_A = "4 word"
-definition L1_index_mask :: address where "L1_index_mask = 0b1111000000"
+definition L1_index_mask :: machine_word where "L1_index_mask = 0b1111000000"
 definition L1_index_offset :: nat where "L1_index_offset = 6"
 type_synonym L2_tag_A = "18 word"
-definition L2_tag_mask :: address where "L2_tag_mask = 0b11111111111111111100000000000000"
+definition L2_tag_mask :: machine_word where "L2_tag_mask = 0b11111111111111111100000000000000"
 definition L2_tag_offset :: nat where "L2_tag_offset = 14"
 type_synonym L2_index_A = "6 word"
-definition L2_index_mask :: address where "L2_index_mask = 0b11111100000000"
+definition L2_index_mask :: machine_word where "L2_index_mask = 0b11111100000000"
 definition L2_index_offset :: nat where "L2_index_offset = 8"
 type_synonym colour_A = "2 word"
-definition colour_mask :: address where "colour_mask = 0b11000000000000"
+definition colour_mask :: machine_word where "colour_mask = 0b11000000000000"
 definition colour_offset :: nat where "colour_offset = 12"
 
-definition L1_tag_of :: "address \<Rightarrow> L1_tag_A" where
-  "L1_tag_of a = ucast ((a AND L1_tag_mask) >> L1_tag_offset)"
-definition L1_index_of :: "address \<Rightarrow> L1_index_A" where
-  "L1_index_of a = ucast ((a AND L1_index_mask) >> L1_index_offset)"
-definition L2_tag_of :: "address \<Rightarrow> L2_tag_A" where
-  "L2_tag_of a = ucast ((a AND L2_tag_mask) >> L2_tag_offset)"
-definition L2_index_of :: "address \<Rightarrow> L2_index_A" where
-  "L2_index_of a = ucast ((a AND L2_index_mask) >> L2_index_offset)"
-definition colour_of :: "address \<Rightarrow> colour_A" where
-  "colour_of a = ucast ((a AND colour_mask) >> colour_offset)"
+definition L1_tag_of :: "vaddr \<Rightarrow> L1_tag_A" where
+  "L1_tag_of a' \<equiv> case a' of VAddr a \<Rightarrow> ucast ((a AND L1_tag_mask) >> L1_tag_offset)"
+definition L1_index_of :: "vaddr \<Rightarrow> L1_index_A" where
+  "L1_index_of a' \<equiv> case a' of VAddr a \<Rightarrow> ucast ((a AND L1_index_mask) >> L1_index_offset)"
+definition L2_tag_of :: "paddr \<Rightarrow> L2_tag_A" where
+  "L2_tag_of a' \<equiv> case a' of PAddr a \<Rightarrow> ucast ((a AND L2_tag_mask) >> L2_tag_offset)"
+definition L2_index_of :: "paddr \<Rightarrow> L2_index_A" where
+  "L2_index_of a' \<equiv> case a' of PAddr a \<Rightarrow> ucast ((a AND L2_index_mask) >> L2_index_offset)"
+definition colour_of :: "paddr \<Rightarrow> colour_A" where
+  "colour_of a' \<equiv> case a' of PAddr a \<Rightarrow> ucast ((a AND colour_mask) >> colour_offset)"
+
+(* So it just takes a `simp` to get rid of the constructor case-split *)
+declare paddr.splits [split]
+declare vaddr.splits [split]
 
 (* Some more made-up numbers. *)
 definition L1_fetch_cycles :: nat where "L1_fetch_cycles = 2"
@@ -79,22 +83,22 @@ definition Default_cycle :: nat where "Default_cycle = 1"
 (* In this system let's choose to have the max number of user domains possible on the hardware
    - that is, as many as there are colours. -robs. *)
 type_synonym userdomain_A = colour_A
-abbreviation addr_colour_A :: "address \<Rightarrow> colour_A" where "addr_colour_A \<equiv> colour_of"
+abbreviation addr_colour_A :: "paddr \<Rightarrow> colour_A" where "addr_colour_A \<equiv> colour_of"
 abbreviation colour_userdomain_A :: "colour_A \<Rightarrow> userdomain_A" where "colour_userdomain_A \<equiv> id"
 
 datatype sys_mode = KEntry | KSchedule | KExit
 
 record orig_state_A =
-  mem :: "address \<Rightarrow> machine_word"
+  mem :: "paddr \<Rightarrow> machine_word"
   curdom :: "userdomain_A domain"
-  taddrs :: "address set"
+  taddrs :: "vaddr set"
 
 type_synonym other_state_A = "orig_state_A \<times> sys_mode"
 
 record regs_A =
   r0 :: "machine_word"
 
-definition collides_in_pch_A :: "address rel" where
+definition collides_in_pch_A :: "paddr rel" where
   "collides_in_pch_A = {(a, a'). L2_index_of a = L2_index_of a'}"
 
 lemma collides_with_equiv_A: "equiv UNIV collides_in_pch_A"
@@ -138,14 +142,14 @@ definition fch_access_impact_A :: "fch_A fch_impact" where
 (* In this case the L1 is writethrough, so we don't need to consult it.
   If it were writeback, we would have to check the dirty bit of any block evicted from it
   to propagate it to the L2 if it is set. *)
-definition pch_read_impact_A :: "(fch_A, pch_A) pch_impact" where
-  "pch_read_impact_A a _ p \<equiv>
+definition pch_read_impact_A :: "pch_A pch_impact" where
+  "pch_read_impact_A a p \<equiv>
      if \<exists> dirty. p (L2_index_of a) = Some (L2_tag_of a, dirty)
        then p
        else p(L2_index_of a := Some (L2_tag_of a, False))"
 
 lemma pch_partitioned_read_A:
-  "(a1, a2) \<notin> collides_in_pch_A \<Longrightarrow> pch_lookup_A p a2 = pch_lookup_A (pch_read_impact_A a1 f p) a2"
+  "(a1, a2) \<notin> collides_in_pch_A \<Longrightarrow> pch_lookup_A p a2 = pch_lookup_A (pch_read_impact_A a1 p) a2"
   unfolding collides_in_pch_A_def pch_lookup_A_def pch_read_impact_A_def
   by auto
 
@@ -155,7 +159,7 @@ lemma pch_collision_read_A:
     set_lookup_eq:
       "\<forall>a3. (a2, a3) \<in> collides_in_pch_A \<longrightarrow> pch_lookup_A pchs a3 = pch_lookup_A pcht a3"
   shows
-    "pch_lookup_A (pch_read_impact_A a1 f pchs) a2 = pch_lookup_A (pch_read_impact_A a1 f pcht) a2"
+    "pch_lookup_A (pch_read_impact_A a1 pchs) a2 = pch_lookup_A (pch_read_impact_A a1 pcht) a2"
   proof -
     have "pch_lookup_A pchs a1 = pch_lookup_A pcht a1 \<and>
           pch_lookup_A pchs a2 = pch_lookup_A pcht a2"
@@ -166,11 +170,11 @@ lemma pch_collision_read_A:
 qed
 
 (* As the L1 is writethrough, we always set the block's dirty bit in the L2 immediately. *)
-definition pch_write_impact_A :: "(fch_A, pch_A) pch_impact" where
-  "pch_write_impact_A a f p \<equiv> p(L2_index_of a := Some (L2_tag_of a, True))"
+definition pch_write_impact_A :: "pch_A pch_impact" where
+  "pch_write_impact_A a p \<equiv> p(L2_index_of a := Some (L2_tag_of a, True))"
 
 lemma pch_partitioned_write_A:
-  "(a1, a2) \<notin> collides_in_pch_A \<Longrightarrow> pch_lookup_A p a2 = pch_lookup_A (pch_write_impact_A a1 f p) a2"
+  "(a1, a2) \<notin> collides_in_pch_A \<Longrightarrow> pch_lookup_A p a2 = pch_lookup_A (pch_write_impact_A a1 p) a2"
   unfolding collides_in_pch_A_def pch_lookup_A_def pch_write_impact_A_def
   by auto
 
@@ -180,7 +184,7 @@ lemma pch_collision_write_A:
     set_lookup_eq:
       "\<forall>a3. (a2, a3) \<in> collides_in_pch_A \<longrightarrow> pch_lookup_A pchs a3 = pch_lookup_A pcht a3"
   shows
-    "pch_lookup_A (pch_write_impact_A a1 f pchs) a2 = pch_lookup_A (pch_write_impact_A a1 f pcht) a2"
+    "pch_lookup_A (pch_write_impact_A a1 pchs) a2 = pch_lookup_A (pch_write_impact_A a1 pcht) a2"
   proof -
     have "pch_lookup_A pchs a1 = pch_lookup_A pcht a1 \<and>
           pch_lookup_A pchs a2 = pch_lookup_A pcht a2"
@@ -198,11 +202,14 @@ definition read_cycles_A :: "fch_cachedness_A \<Rightarrow> pch_cachedness_A \<R
 definition write_cycles_A :: "fch_cachedness_A \<Rightarrow> pch_cachedness_A \<Rightarrow> time" where
   "write_cycles_A _ _ = Default_cycle"
 
-definition do_read_A :: "address \<Rightarrow> other_state_A \<Rightarrow> regs_A \<Rightarrow> regs_A" where
-  "do_read_A a s _ = \<lparr> r0 = mem (fst s) a \<rparr>"
+definition v_to_p_A :: "other_state_A \<Rightarrow> vaddr \<Rightarrow> paddr" where
+  "v_to_p_A s v \<equiv> case v of VAddr a \<Rightarrow> PAddr a" (* id just to get the types to line up first *)
 
-definition do_write_A :: "address \<Rightarrow> other_state_A \<Rightarrow> regs_A \<Rightarrow> other_state_A" where
-  "do_write_A a s rs = ((fst s)\<lparr> mem := (mem (fst s))(a := r0 rs) \<rparr>, snd s)"
+definition do_read_A :: "vaddr \<Rightarrow> other_state_A \<Rightarrow> regs_A \<Rightarrow> regs_A" where
+  "do_read_A a s _ = \<lparr> r0 = mem (fst s) (v_to_p_A s a) \<rparr>"
+
+definition do_write_A :: "vaddr \<Rightarrow> other_state_A \<Rightarrow> regs_A \<Rightarrow> other_state_A" where
+  "do_write_A a s rs = ((fst s)\<lparr> mem := (mem (fst s))(v_to_p_A s a := r0 rs) \<rparr>, snd s)"
 
 definition store_time_A :: "time \<Rightarrow> regs_A \<Rightarrow> regs_A" where
   "store_time_A t r = \<lparr> r0 = of_nat t \<rparr>"
@@ -220,17 +227,17 @@ definition empty_fch_A :: fch_A where
 definition fch_flush_cycles_A:: "fch_A \<Rightarrow> time" where
   "fch_flush_cycles_A _ = Default_cycle"
 
-definition L2_indices_of :: "address set \<Rightarrow> L2_index_A set" where
+definition L2_indices_of :: "paddr set \<Rightarrow> L2_index_A set" where
   "L2_indices_of as \<equiv> {idx. \<exists> a. L2_index_of a = idx \<and> a \<in> as}"
 
-definition do_pch_flush_A :: "pch_A \<Rightarrow> address set \<Rightarrow> pch_A" where
+definition do_pch_flush_A :: "pch_A \<Rightarrow> paddr set \<Rightarrow> pch_A" where
   "do_pch_flush_A p as \<equiv> \<lambda> idx. if idx \<in> L2_indices_of as then None else p idx"
 
 (* Let's say the flush time is proportional to the number of sets we're asking to be flushed
    -- to begin with, *not* sensitive to the current cachedness status of those sets.
    We may later want to try this for manual flushing schemes whose timing might depend on
    whether each index has an entry loaded in the cache or not, whether it is dirty, etc. *)
-definition pch_flush_cycles_A :: "pch_A \<Rightarrow> address set \<Rightarrow> time" where
+definition pch_flush_cycles_A :: "pch_A \<Rightarrow> paddr set \<Rightarrow> time" where
   "pch_flush_cycles_A p as = Default_cycle + length (sorted_list_of_set (L2_indices_of as))"
 
 lemma pch_partitioned_flush_A:
@@ -256,13 +263,14 @@ lemma pch_flush_cycles_localised_A:
   (* By this flush_cycles definition, we don't need the assumption after all. *)
   by (clarsimp simp:pch_flush_cycles_A_def)
 
-definition addr_domain_A :: "address \<Rightarrow> userdomain_A domain" where
+definition addr_domain_A :: "paddr \<Rightarrow> userdomain_A domain" where
   "addr_domain_A a = User (colour_userdomain_A (addr_colour_A a))"
 
 lemma same_index_same_colour:
   "L2_index_of a = L2_index_of b \<Longrightarrow> colour_of a = colour_of b"
   unfolding L2_index_of_def colour_of_def
     L2_index_mask_def L2_index_offset_def colour_mask_def colour_offset_def
+  apply simp
   by (word_bitwise, simp)
 
 lemma no_cross_colour_collisions_A:
@@ -301,21 +309,31 @@ lemma external_uwr_same_domain_A:
   "(s1, s2) \<in> external_uwr_A d \<Longrightarrow> current_domain_A s1 = current_domain_A s2"
   unfolding external_uwr_A_def current_domain_A_def by blast
 
+lemma page_table_not_in_mem_A:
+  "\<And>a s r. v_to_p_A (do_write_A a s r) = v_to_p_A s"
+  unfolding v_to_p_A_def do_write_A_def
+  by blast
+
+lemma external_uwr_current_page_table_A:
+  "(s1, s2) \<in> external_uwr_A d \<Longrightarrow> current_domain_A s1 = d \<Longrightarrow> v_to_p_A s1 = v_to_p_A s2"
+  unfolding external_uwr_A_def current_domain_A_def v_to_p_A_def
+  by blast
+
 lemma do_write_maintains_external_uwr_out_A:
-  "addr_domain_A a \<noteq> d \<and> addr_domain_A a \<noteq> Sched \<Longrightarrow>
+  "addr_domain_A (v_to_p_A s a) \<noteq> d \<and> addr_domain_A (v_to_p_A s a) \<noteq> Sched \<Longrightarrow>
    (s, do_write_A a s r) \<in> external_uwr_A d"
   unfolding do_write_A_def external_uwr_A_def
   by force
 
 lemma do_write_maintains_external_uwr_in_A:
-  "addr_domain_A a = d \<or> addr_domain_A a = Sched \<Longrightarrow>
+  "addr_domain_A (v_to_p_A s a) = d \<or> addr_domain_A (v_to_p_A s a) = Sched \<Longrightarrow>
    (s, t) \<in> external_uwr_A d \<Longrightarrow>
    (do_write_A a s r, do_write_A a t r) \<in> external_uwr_A d"
-  unfolding do_write_A_def external_uwr_A_def
+  unfolding do_write_A_def external_uwr_A_def v_to_p_A_def
   by force
 
 lemma do_write_outside_kernelshared_same_domain_A:
-  assumes "addr_domain_A a \<noteq> Sched"
+  assumes "addr_domain_A (v_to_p_A s a) \<noteq> Sched"
   shows "current_domain_A (do_write_A a s r) = current_domain_A s"
   (* Note: We didn't need the assumption *)
   unfolding current_domain_A_def do_write_A_def
@@ -323,19 +341,19 @@ lemma do_write_outside_kernelshared_same_domain_A:
 
 lemma do_read_from_external_uwr_domain_A:
   "\<lbrakk>(s, t) \<in> external_uwr_A d;
-   addr_domain_A a = d \<rbrakk> \<Longrightarrow>
+   addr_domain_A (v_to_p_A s a) = d \<rbrakk> \<Longrightarrow>
    do_read_A a s r = do_read_A a t r"
-  unfolding external_uwr_A_def do_read_A_def
+  unfolding external_uwr_A_def do_read_A_def v_to_p_A_def
   by force
 
 lemma do_read_from_external_uwr_sched_A:
   "\<lbrakk>(s, t) \<in> external_uwr_A d;
-   addr_domain_A a = Sched \<rbrakk> \<Longrightarrow>
+   addr_domain_A (v_to_p_A s a) = Sched \<rbrakk> \<Longrightarrow>
    do_read_A a s r = do_read_A a t r"
-  unfolding external_uwr_A_def do_read_A_def
+  unfolding external_uwr_A_def do_read_A_def v_to_p_A_def
   by force
 
-definition touched_addrs_A :: "other_state_A \<Rightarrow> address set" where
+definition touched_addrs_A :: "other_state_A \<Rightarrow> vaddr set" where
   "touched_addrs_A s = taddrs (fst s)"
 
 lemma external_uwr_same_touched_addrs_A:
@@ -343,6 +361,71 @@ lemma external_uwr_same_touched_addrs_A:
    touched_addrs_A s1 = touched_addrs_A s2"
   unfolding external_uwr_A_def current_domain_A_def touched_addrs_A_def
   by blast
+
+lemma touched_addrs_not_in_mem_A:
+  "\<And>a s r. touched_addrs_A (do_write_A a s r) = touched_addrs_A s"
+  unfolding touched_addrs_A_def do_write_A_def
+  by force
+ 
+definition do_add_to_TA_A :: "other_state_A \<Rightarrow> vaddr set \<Rightarrow> other_state_A" where
+  "do_add_to_TA_A s vas \<equiv> (fst s \<lparr> taddrs := taddrs (fst s) \<union> vas \<rparr>, snd s)"
+
+lemma do_add_to_TA_correct_A:
+  "\<And>s vas. touched_addrs_A (do_add_to_TA_A s vas) = touched_addrs_A s \<union> vas"
+  "\<And>s vas. current_domain_A (do_add_to_TA_A s vas) = current_domain_A s"
+  "\<And>s vas. v_to_p_A (do_add_to_TA_A s vas) = v_to_p_A s"
+  apply -
+    unfolding touched_addrs_A_def do_add_to_TA_A_def
+    apply force
+   unfolding current_domain_A_def
+   apply force
+  unfolding v_to_p_A_def
+  by blast
+
+lemma do_add_to_TA_maintains_external_uwr_in_A:
+  "\<And>s t d vas.
+     (s, t) \<in> external_uwr_A d \<Longrightarrow>
+     current_domain_A s = d \<Longrightarrow>
+     (do_add_to_TA_A s vas, do_add_to_TA_A t vas) \<in> external_uwr_A d"
+  unfolding external_uwr_A_def current_domain_A_def do_add_to_TA_A_def
+  by force
+
+lemma do_add_to_TA_maintains_external_uwr_out_A:
+  "\<And>s vas.
+     current_domain_A s \<noteq> d \<Longrightarrow>
+     (s, do_add_to_TA_A s vas) \<in> external_uwr_A d"
+  unfolding external_uwr_A_def current_domain_A_def do_add_to_TA_A_def
+  by force
+
+definition do_empty_TA_A :: "other_state_A \<Rightarrow> other_state_A" where
+  "do_empty_TA_A s \<equiv> (fst s \<lparr> taddrs := {} \<rparr>, snd s)"
+
+lemma do_empty_TA_correct_A:
+  "\<And>s. touched_addrs_A (do_empty_TA_A s) = {}"
+  "\<And>s. current_domain_A (do_empty_TA_A s) = current_domain_A s"
+  "\<And>s. v_to_p_A (do_empty_TA_A s) = v_to_p_A s"
+    apply -
+    unfolding touched_addrs_A_def do_empty_TA_A_def
+    apply force
+   unfolding current_domain_A_def
+   apply force
+  unfolding v_to_p_A_def
+  by blast
+
+lemma do_empty_TA_maintains_external_uwr_in_A:
+  "\<And>s t d.
+     (s, t) \<in> external_uwr_A d \<Longrightarrow>
+     current_domain_A s = d \<Longrightarrow>
+     (do_empty_TA_A s, do_empty_TA_A t) \<in> external_uwr_A d"
+  unfolding external_uwr_A_def current_domain_A_def do_empty_TA_A_def
+  by force
+
+lemma do_empty_TA_maintains_external_uwr_out_A:
+  "\<And>s.
+     current_domain_A s \<noteq> d \<Longrightarrow>
+     (s, do_empty_TA_A s) \<in> external_uwr_A d"
+  unfolding external_uwr_A_def current_domain_A_def do_empty_TA_A_def
+  by force
 
 definition can_domain_switch_A :: "other_state_A \<Rightarrow> bool" where
   "can_domain_switch_A s \<equiv> snd s = KSchedule"
@@ -361,27 +444,40 @@ interpretation time_protection_A: time_protection collides_in_pch_A
   store_time_A padding_regs_impact_A
   empty_fch_A fch_flush_cycles_A do_pch_flush_A pch_flush_cycles_A
   addr_domain_A addr_colour_A colour_userdomain_A
-  current_domain_A external_uwr_A touched_addrs_A can_domain_switch_A
+  current_domain_A external_uwr_A v_to_p_A touched_addrs_A
+  do_add_to_TA_A do_empty_TA_A
+  can_domain_switch_A
   apply unfold_locales
-                    using collides_with_equiv_A apply blast
-                   using pch_partitioned_read_A apply blast
-                  using pch_collision_read_A apply blast
-                 using pch_partitioned_write_A apply blast
-                using pch_collision_write_A apply blast
-               using pch_partitioned_flush_A apply blast
-              using pch_collision_flush_A apply blast
-             using pch_flush_cycles_localised_A apply blast
-            using no_cross_colour_collisions_A apply blast
-           using addr_domain_valid_A apply blast
-          using external_uwr_equiv_rel_A apply blast
-         using external_uwr_same_domain_A apply blast
-        using do_write_maintains_external_uwr_out_A apply blast
-       using do_write_maintains_external_uwr_in_A apply blast
-      using do_write_outside_kernelshared_same_domain_A apply blast
-     using do_read_from_external_uwr_domain_A apply blast
+    (* Forget the indentation: it'll just keep fluctuating as we experiment
+       with the interface -robs. *)
+    using collides_with_equiv_A apply blast
+    using pch_partitioned_read_A apply blast
+    using pch_collision_read_A apply blast
+    using pch_partitioned_write_A apply blast
+    using pch_collision_write_A apply blast
+    using pch_partitioned_flush_A apply blast
+    using pch_collision_flush_A apply blast
+    using pch_flush_cycles_localised_A apply blast
+    using no_cross_colour_collisions_A apply blast
+    using addr_domain_valid_A apply blast
+    using external_uwr_equiv_rel_A apply blast
+    using external_uwr_same_domain_A apply blast
+    using page_table_not_in_mem_A apply blast
+    using external_uwr_current_page_table_A apply blast
+    using do_write_maintains_external_uwr_out_A apply blast
+    using do_write_maintains_external_uwr_in_A apply blast
+    using do_write_outside_kernelshared_same_domain_A apply blast
+    using do_read_from_external_uwr_domain_A apply blast
     using do_read_from_external_uwr_sched_A apply blast
-   using external_uwr_same_touched_addrs_A apply blast
-  using can_domain_switch_public_A apply blast
+    using external_uwr_same_touched_addrs_A apply blast
+    using touched_addrs_not_in_mem_A apply blast
+    using do_add_to_TA_correct_A apply auto[3]
+    using do_add_to_TA_maintains_external_uwr_in_A apply blast
+    using do_add_to_TA_maintains_external_uwr_out_A apply blast
+    using do_empty_TA_correct_A apply auto[3]
+    using do_empty_TA_maintains_external_uwr_in_A apply blast
+    using do_empty_TA_maintains_external_uwr_out_A apply blast
+    using can_domain_switch_public_A apply blast
   done
 (* Gerwin's feedback: at least get to the end of this once
    so we know it's satisfiable even if not flexible *)
@@ -458,8 +554,8 @@ interpretation time_protection_refinement_A: time_protection_refinement
   do_read_A do_write_A
   store_time_A padding_regs_impact_A
   empty_fch_A fch_flush_cycles_A do_pch_flush_A pch_flush_cycles_A
-  addr_domain_A addr_colour_A colour_userdomain_A
-  touched_addrs_A can_domain_switch_A
+  addr_domain_A addr_colour_A colour_userdomain_A v_to_p_A
+  touched_addrs_A do_add_to_TA_A do_empty_TA_A can_domain_switch_A
   initial_regs_A initial_pch_A
   refined_step_to_program (* TODO *)
   apply unfold_locales
